src/tls/Extensions.fsti
@@ -1,0 +1,241 @@
+(* Copyright (C) 2012--2017 Microsoft Research and INRIA *)
+(**
+This modules defines TLS 1.3 Extensions.
+
+- An AST, and it's associated parsing and formatting functions.
+- Nego calls prepareExtensions : config -> list extensions.
+
+@summary: TLS 1.3 Extensions.
+*)
+module Extensions
+
+open FStar.Bytes
+open FStar.Error
+open TLSError
+open TLSConstants
+
+(*************************************************
+ Define extension.
+ *************************************************)
+// Extensions may appear in the following messages
+// The concrete message syntax
+type ext_msg =
+  | EM_ClientHello
+  | EM_ServerHello
+  | EM_EncryptedExtensions
+  | EM_Certificate
+  | EM_NewSessionTicket
+  | EM_HelloRetryRequest
+
+(* As a static invariant, we record that any intermediate, parsed
+extension and extension lists can be formatted into bytes without
+overflowing 2^16. This create dependencies on the formatting
+functions, at odd with recursive extensions. *)
+
+(* PRE-SHARED KEYS AND KEY EXCHANGES *)
+type pskIdentity = PSK.psk_identifier * PSK.obfuscated_ticket_age
+
+val pskiBytes: PSK.psk_identifier * PSK.obfuscated_ticket_age -> bytes
+val pskiListBytes: list pskIdentity -> bytes
+
+noeq type psk =
+  // this is the truncated PSK extension, without the list of binder tags.
+  | ClientPSK:
+    identities:list pskIdentity{
+      let n = length (pskiListBytes identities) in 6 < n /\ n < 65536} ->
+    binders_len:nat{binders_len <= 65535} ->
+    psk
+  // this is just an index in the client offer's PSK extension
+  | ServerPSK: UInt16.t -> psk
+
+// PSK binders, actually the truncated suffix of TLS 1.3 ClientHello
+// We statically enforce length requirements to ensure that formatting is total.
+type binder = b:bytes {32 <= length b /\ length b <= 255}
+
+(** REMARK: this is more restrictive than in the RFC, which allows up to 2047 binders *)
+type binders =
+  bs:list binder {1 <= List.Tot.length bs /\ List.Tot.length bs < 255}
+
+val bindersBytes: bs:binders -> b:bytes{length b >= 35 /\ length b <= 65537}
+
+// https://tlswg.github.io/tls13-spec/#rfc.section.4.2.8
+// restricting both proposed PSKs and future ones sent by the server
+// will also be used in the PSK table, and possibly in the configs
+type psk_kex =
+  | PSK_KE
+  | PSK_DHE_KE
+
+type client_psk_kexes = l:list psk_kex
+  { l = [PSK_KE] \/ l = [PSK_DHE_KE] \/ l = [PSK_KE; PSK_DHE_KE] \/ l = [PSK_DHE_KE; PSK_KE] }
+
+let client_psk_kexes_length (l:client_psk_kexes): Lemma (List.Tot.length l < 3) = ()
+
+
+type earlyDataIndication = option UInt32.t // Some  max_early_data_size, only in  NewSessionTicket
+
+// used by QUIC interface too
+val quicParametersBytes_aux: pl:list quicParameter -> b:bytes{length b <= op_Multiply (List.Tot.length pl) 256}
+val parseQuicParameters_aux: bytes -> result (list quicParameter)
+
+// The length exactly reflects the RFC format constraint <2..254>
+type protocol_versions =
+  | ServerPV of protocolVersion
+  | ClientPV of l:list protocolVersion {0 < List.Tot.length l /\ List.Tot.length l < 128}
+
+
+// ExtensionType and Extension Table in https://tlswg.github.io/tls13-spec/#rfc.section.4.2.
+// M=Mandatory, AF=mandatory for Application Features in https://tlswg.github.io/tls13-spec/#rfc.section.8.2.
+noeq type extension' (p: (lbytes 2 -> GTot Type0)) =
+  | E_server_name of list serverName (* M, AF *) (* RFC 6066 *)
+  | E_supported_groups of list namedGroup (* M, AF *) (* RFC 7919 *)
+  | E_signature_algorithms of signatureSchemeList (* M, AF *) (* RFC 5246 *)
+  | E_signature_algorithms_cert of signatureSchemeList (* TLS 1.3#23 addition; TLS 1.2 should also support it *)
+  | E_key_share of CommonDH.keyShare (* M, AF *)
+  | E_pre_shared_key of psk (* M, AF *)
+  | E_session_ticket of bytes
+  | E_early_data of earlyDataIndication
+  | E_supported_versions of protocol_versions   (* M, AF *)
+  | E_cookie of b:bytes {0 < length b /\ length b < 65536}  (* M *)
+  | E_psk_key_exchange_modes of client_psk_kexes (* client-only; mandatory when proposing PSKs *)
+  | E_extended_ms
+  | E_ec_point_format of list point_format
+  | E_alpn of alpn
+  | E_quic_parameters of quicParameters
+  | E_unknown_extension of ((x: lbytes 2 {p x}) * bytes) (* header, payload *)
+(*
+We do not yet support the extensions below (authenticated but ignored)
+  | E_max_fragment_length
+  | E_status_request
+  | E_use_srtp
+  | E_heartbeat
+  | E_signed_certifcate_timestamp
+  | E_client_certificate_type
+  | E_server_certificate_type
+  | E_certificate_authorities
+  | E_oid_filters
+  | E_post_handshake_auth
+  | E_renegotiation_info of renegotiationInfo
+*)
+
+type knownTag = lbytes 2 -> GTot Type0
+val bindersLen: #p: knownTag -> el: list (extension' p) -> nat 
+val string_of_extension: #p: knownTag -> extension' p -> string 
+val string_of_extensions: #p: knownTag -> list (extension' p) -> string 
+
+(** shallow equality, comparing just the extension tags *)
+val sameExt: #p: knownTag -> e1: extension' p -> e2: extension' p -> bool
+
+(*************************************************
+ extension formatting
+ *************************************************)
+
+val extensionHeaderBytes: #p: knownTag -> extension' p -> lbytes 2
+
+// 17-05-19: We constrain unknown extensions to have headers different from known extensions.
+let unknown_extensions_unknown (h: lbytes 2): GTot Type0 = 
+  forall (p: knownTag) (e' : extension' p { h=extensionHeaderBytes e' } ) . E_unknown_extension? e'
+
+type extension = extension' unknown_extensions_unknown
+
+let encryptedExtension (ext: extension): bool =
+  match ext with
+  | E_server_name _
+  | E_supported_groups _
+  | E_alpn _
+  | E_quic_parameters _
+  | E_early_data _ -> true
+  | _ -> false
+
+
+(** Serializes an extension *)
+val extensionBytes: ext:extension -> b:bytes { 2 <= length b /\ length b < 65536 }
+val extensionBytes_is_injective: 
+  ext1: extension -> s1: bytes ->
+  ext2: extension -> s2: bytes -> Lemma
+  (requires (Bytes.equal (extensionBytes ext1 @| s1) (extensionBytes ext2 @| s2)))
+  (ensures (ext1 == ext2 /\ s1 == s2))
+
+// we'll need to reveal more to build extensions...
+val extensionListBytes: exts: list extension -> bytes
+type extensions = exts:list extension {repr_bytes (length (extensionListBytes exts)) <= 2}
+
+(** Serializes a list of extensions.
+  If there is a PreSharedKey client extension, then add the length of the PSK binders to
+  the total length. Note that the `E_pre_shared_key` argument includes the length of
+  binders in this case.
+*)
+
+type valid_extensions = exts: extensions {length (extensionListBytes exts) + bindersLen exts < 65536}
+
+val extensionsBytes:
+  exts:valid_extensions -> b:bytes {2 <= length b /\ length b < 2 + 65536}
+
+val extensionsBytes_is_injective_strong:
+  exts1:valid_extensions -> s1: bytes ->
+  exts2:valid_extensions -> s2: bytes -> Lemma
+  (requires Bytes.equal (extensionsBytes exts1 @| s1) (extensionsBytes exts2 @| s2))
+  (ensures exts1 == exts2 /\ s1 == s2)
+
+val extensionsBytes_is_injective:
+  ext1:valid_extensions ->
+  ext2:valid_extensions -> Lemma 
+  (requires Bytes.equal (extensionsBytes ext1) (extensionsBytes ext2))
+  (ensures ext1 == ext2)
+
+(*************************************************
+ Extension parsing
+**************************************************)
+
+val parseExtension:     ext_msg -> bytes -> result (extension * option binders)
+val parseExtensions:    ext_msg -> bytes -> result (extensions * option binders)
+val parseOptExtensions: ext_msg -> bytes -> result (option (list extension) * option binders)
+
+(*************************************************
+ Other extension functionality
+ *************************************************)
+
+/// 18-02-21 the rest of this module has nothing to do with formats,
+/// could go to Negotiation or to a new Nego.Extensions module
+
+val prepareExtensions:
+  protocolVersion ->
+  protocolVersion ->
+  k:valid_cipher_suites{List.Tot.length k < 256} ->
+  option bytes -> // SNI
+  option alpn -> // ALPN
+  option quicParameters ->
+  bool -> // EMS
+  bool ->
+  bool -> // EDI (Nego checks that PSK is compatible)
+  option bytes -> // session_ticket
+  signatureSchemeList ->
+  list valid_namedGroup ->
+  option (cVerifyData * sVerifyData) ->
+  option CommonDH.keyShare ->
+  list (PSK.pskid * pskInfo) ->
+  l:list extension{List.Tot.length l < 256}
+
+val negotiateClientExtensions:
+  protocolVersion ->
+  config ->
+  option (list extension) ->
+  option (list extension) ->
+  cipherSuite ->
+  option (cVerifyData * sVerifyData) ->
+  bool ->
+  result protocolVersion
+
+val negotiateServerExtensions: 
+  protocolVersion -> 
+  option (list extension) -> 
+  valid_cipher_suites -> 
+  config -> 
+  cipherSuite -> 
+  option (cVerifyData * sVerifyData) -> 
+  option nat -> 
+  option CommonDH.keyShare -> 
+  bool -> 
+  result (option (list extension))
+
+val default_signatureScheme: 
+  protocolVersion -> cipherSuite -> ML signatureSchemeList
